theories/FSets/FSetList.v
@@ -6,7 +6,7 @@
 (*         *       GNU Lesser General Public License Version 2.1       *)
 (***********************************************************************)
 
-(* $Id: FSetList.v,v 1.12 2006/03/10 10:49:48 letouzey Exp $ *)
+(* $Id$ *)
 
 (** * Finite sets library *)
 
@@ -23,25 +23,25 @@ Unset Strict Implicit.
    The specs are proved under the additional condition of being sorted. 
    And the functions returning sets are proved to preserve this invariant. *)
 
-Module Raw (X: OrderedType).
+Module Raw (X OrderedType).
  
-  Module E := X.
-  Module MX := OrderedTypeFacts X.
+  Module E = X.
+  Module MX = OrderedTypeFacts X.
   Import MX.
 
-  Definition elt := X.t.
-  Definition t := list elt.
+  Definition elt = X.t.
+  Definition t = list elt.
 
-  Definition empty : t := nil.
+  Definition empty  t := nil.
 
-  Definition is_empty (l : t) : bool := if l then true else false.
+  Definition is_empty (l  t) : bool := if l then true else false.
 
   (** ** The set operations. *)
 
-  Fixpoint mem (x : elt) (s : t) {struct s} : bool :=
+  Fixpoint mem (x  elt) (s : t) {struct s} : bool :=
     match s with
     | nil => false
-    | y :: l =>
+    | y : l =>
         match X.compare x y with
         | Lt _ => false
         | Eq _ => true
@@ -49,83 +49,83 @@ Module Raw (X: OrderedType).
         end
     end.
 
-  Fixpoint add (x : elt) (s : t) {struct s} : t :=
+  Fixpoint add (x  elt) (s : t) {struct s} : t :=
     match s with
-    | nil => x :: nil
-    | y :: l =>
+    | nil => x : nil
+    | y : l =>
         match X.compare x y with
-        | Lt _ => x :: s
+        | Lt _ => x : s
         | Eq _ => s
-        | Gt _ => y :: add x l
+        | Gt _ => y : add x l
         end
     end.
 
-  Definition singleton (x : elt) : t := x :: nil. 
+  Definition singleton (x  elt) : t := x :: nil. 
 
-  Fixpoint remove (x : elt) (s : t) {struct s} : t :=
+  Fixpoint remove (x  elt) (s : t) {struct s} : t :=
     match s with
     | nil => nil
-    | y :: l =>
+    | y : l =>
         match X.compare x y with
         | Lt _ => s
         | Eq _ => l
-        | Gt _ => y :: remove x l
+        | Gt _ => y : remove x l
         end
     end.  
   
-  Fixpoint union (s : t) : t -> t :=
+  Fixpoint union (s  t) : t -> t :=
     match s with
     | nil => fun s' => s'
-    | x :: l =>
-        (fix union_aux (s' : t) : t :=
+    | x : l =>
+        (fix union_aux (s'  t) : t :=
            match s' with
            | nil => s
-           | x' :: l' =>
+           | x' : l' =>
                match X.compare x x' with
-               | Lt _ => x :: union l s'
-               | Eq _ => x :: union l l'
-               | Gt _ => x' :: union_aux l'
+               | Lt _ => x : union l s'
+               | Eq _ => x : union l l'
+               | Gt _ => x' : union_aux l'
                end
            end)
     end.      
 
-  Fixpoint inter (s : t) : t -> t :=
+  Fixpoint inter (s  t) : t -> t :=
     match s with
     | nil => fun _ => nil
-    | x :: l =>
-        (fix inter_aux (s' : t) : t :=
+    | x : l =>
+        (fix inter_aux (s'  t) : t :=
            match s' with
            | nil => nil
-           | x' :: l' =>
+           | x' : l' =>
                match X.compare x x' with
                | Lt _ => inter l s'
-               | Eq _ => x :: inter l l'
+               | Eq _ => x : inter l l'
                | Gt _ => inter_aux l'
                end
            end)
     end.  
   
-  Fixpoint diff (s : t) : t -> t :=
+  Fixpoint diff (s  t) : t -> t :=
     match s with
     | nil => fun _ => nil
-    | x :: l =>
-        (fix diff_aux (s' : t) : t :=
+    | x : l =>
+        (fix diff_aux (s'  t) : t :=
            match s' with
            | nil => s
-           | x' :: l' =>
+           | x' : l' =>
                match X.compare x x' with
-               | Lt _ => x :: diff l s'
+               | Lt _ => x : diff l s'
                | Eq _ => diff l l'
                | Gt _ => diff_aux l'
                end
            end)
     end.  
    
-  Fixpoint equal (s : t) : t -> bool :=
-    fun s' : t =>
+  Fixpoint equal (s  t) : t -> bool :=
+    fun s'  t =>
     match s, s' with
     | nil, nil => true
-    | x :: l, x' :: l' =>
+    | x : l, x' :: l' =>
         match X.compare x x' with
         | Eq _ => equal l l'
         | _ => false
@@ -133,10 +133,10 @@ Module Raw (X: OrderedType).
     | _, _ => false
     end.
 
-  Fixpoint subset (s s' : t) {struct s'} : bool :=
+  Fixpoint subset (s s'  t) {struct s'} : bool :=
     match s, s' with
     | nil, _ => true
-    | x :: l, x' :: l' =>
+    | x : l, x' :: l' =>
         match X.compare x x' with
         | Lt _ => false
         | Eq _ => subset l l'
@@ -145,72 +145,72 @@ Module Raw (X: OrderedType).
     | _, _ => false
     end.
 
-  Fixpoint fold (B : Set) (f : elt -> B -> B) (s : t) {struct s} : 
-   B -> B := fun i => match s with
+  Fixpoint fold (B  Set) (f : elt -> B -> B) (s : t) {struct s} : 
+   B -> B = fun i => match s with
                       | nil => i
-                      | x :: l => fold f l (f x i)
+                      | x : l => fold f l (f x i)
                       end.  
 
-  Fixpoint filter (f : elt -> bool) (s : t) {struct s} : t :=
+  Fixpoint filter (f  elt -> bool) (s : t) {struct s} : t :=
     match s with
     | nil => nil
-    | x :: l => if f x then x :: filter f l else filter f l
+    | x : l => if f x then x :: filter f l else filter f l
     end.  
 
-  Fixpoint for_all (f : elt -> bool) (s : t) {struct s} : bool :=
+  Fixpoint for_all (f  elt -> bool) (s : t) {struct s} : bool :=
     match s with
     | nil => true
-    | x :: l => if f x then for_all f l else false
+    | x : l => if f x then for_all f l else false
     end.  
  
-  Fixpoint exists_ (f : elt -> bool) (s : t) {struct s} : bool :=
+  Fixpoint exists_ (f  elt -> bool) (s : t) {struct s} : bool :=
     match s with
     | nil => false
-    | x :: l => if f x then true else exists_ f l
+    | x : l => if f x then true else exists_ f l
     end.
 
-  Fixpoint partition (f : elt -> bool) (s : t) {struct s} : 
-   t * t :=
+  Fixpoint partition (f  elt -> bool) (s : t) {struct s} : 
+   t * t =
     match s with
     | nil => (nil, nil)
-    | x :: l =>
-        let (s1, s2) := partition f l in
-        if f x then (x :: s1, s2) else (s1, x :: s2)
+    | x : l =>
+        let (s1, s2) = partition f l in
+        if f x then (x : s1, s2) else (s1, x :: s2)
     end.
 
-  Definition cardinal (s : t) : nat := length s.
+  Definition cardinal (s  t) : nat := length s.
 
-  Definition elements (x : t) : list elt := x.
+  Definition elements (x  t) : list elt := x.
 
-  Definition min_elt (s : t) : option elt :=
+  Definition min_elt (s  t) : option elt :=
     match s with
     | nil => None
-    | x :: _ => Some x
+    | x : _ => Some x
     end.
 
-  Fixpoint max_elt (s : t) : option elt :=
+  Fixpoint max_elt (s  t) : option elt :=
     match s with
     | nil => None
-    | x :: nil => Some x
-    | _ :: l => max_elt l
+    | x : nil => Some x
+    | _ : l => max_elt l
     end.
 
-  Definition choose := min_elt.
+  Definition choose = min_elt.
 
   (** ** Proofs of set operation specifications. *)
 
-  Notation Sort := (sort X.lt).
-  Notation Inf := (lelistA X.lt).
-  Notation In := (InA X.eq).
+  Notation Sort = (sort X.lt).
+  Notation Inf = (lelistA X.lt).
+  Notation In = (InA X.eq).
 
-  Definition Equal s s' := forall a : elt, In a s <-> In a s'.
-  Definition Subset s s' := forall a : elt, In a s -> In a s'.
-  Definition Empty s := forall a : elt, ~ In a s.
-  Definition For_all (P : elt -> Prop) s := forall x, In x s -> P x.
-  Definition Exists (P : elt -> Prop) (s : t) := exists x, In x s /\ P x.
+  Definition Equal s s' = forall a : elt, In a s <-> In a s'.
+  Definition Subset s s' = forall a : elt, In a s -> In a s'.
+  Definition Empty s = forall a : elt, ~ In a s.
+  Definition For_all (P  elt -> Prop) s := forall x, In x s -> P x.
+  Definition Exists (P  elt -> Prop) (s : t) := exists x, In x s /\ P x.
 
-  Lemma mem_1 :
-   forall (s : t) (Hs : Sort s) (x : elt), In x s -> mem x s = true. 
+  Lemma mem_1 
+   forall (s  t) (Hs : Sort s) (x : elt), In x s -> mem x s = true. 
   Proof.
   simple induction s; intros.
   inversion H.
@@ -221,7 +221,7 @@ Module Raw (X: OrderedType).
   apply Sort_Inf_In with l; trivial.
   Qed.
 
-  Lemma mem_2 : forall (s : t) (x : elt), mem x s = true -> In x s.
+  Lemma mem_2  forall (s : t) (x : elt), mem x s = true -> In x s.
   Proof.
   simple induction s.
   intros; inversion H.
@@ -230,8 +230,8 @@ Module Raw (X: OrderedType).
   case (X.compare x a); intros; try discriminate; auto.
   Qed.
 
-  Lemma add_Inf :
-   forall (s : t) (x a : elt), Inf a s -> X.lt a x -> Inf a (add x s).
+  Lemma add_Inf 
+   forall (s  t) (x a : elt), Inf a s -> X.lt a x -> Inf a (add x s).
   Proof.
   simple induction s.  
   simpl; intuition.
@@ -240,7 +240,7 @@ Module Raw (X: OrderedType).
   Qed.
   Hint Resolve add_Inf.
   
-  Lemma add_sort : forall (s : t) (Hs : Sort s) (x : elt), Sort (add x s).
+  Lemma add_sort  forall (s : t) (Hs : Sort s) (x : elt), Sort (add x s).
   Proof.
   simple induction s.
   simpl; intuition.
@@ -248,8 +248,8 @@ Module Raw (X: OrderedType).
    auto.
   Qed. 
 
-  Lemma add_1 :
-   forall (s : t) (Hs : Sort s) (x y : elt), X.eq x y -> In y (add x s).
+  Lemma add_1 
+   forall (s  t) (Hs : Sort s) (x y : elt), X.eq x y -> In y (add x s).
   Proof.
   simple induction s. 
   simpl; intuition.
@@ -257,8 +257,8 @@ Module Raw (X: OrderedType).
   constructor; apply X.eq_trans with x; auto.
   Qed.
 
-  Lemma add_2 :
-   forall (s : t) (Hs : Sort s) (x y : elt), In y s -> In y (add x s).
+  Lemma add_2 
+   forall (s  t) (Hs : Sort s) (x y : elt), In y s -> In y (add x s).
   Proof.
   simple induction s. 
   simpl; intuition.
@@ -266,8 +266,8 @@ Module Raw (X: OrderedType).
   inversion_clear Hs; inversion_clear H0; auto.
   Qed.
 
-  Lemma add_3 :
-   forall (s : t) (Hs : Sort s) (x y : elt),
+  Lemma add_3 
+   forall (s  t) (Hs : Sort s) (x y : elt),
    ~ X.eq x y -> In y (add x s) -> In y s.
   Proof.
   simple induction s. 
@@ -278,8 +278,8 @@ Module Raw (X: OrderedType).
   constructor 2; apply Hrec with x; auto.
   Qed.
 
-  Lemma remove_Inf :
-   forall (s : t) (Hs : Sort s) (x a : elt), Inf a s -> Inf a (remove x s).
+  Lemma remove_Inf 
+   forall (s  t) (Hs : Sort s) (x a : elt), Inf a s -> Inf a (remove x s).
   Proof.
   simple induction s.  
   simpl; intuition.
@@ -288,16 +288,16 @@ Module Raw (X: OrderedType).
   Qed.
   Hint Resolve remove_Inf.
 
-  Lemma remove_sort :
-   forall (s : t) (Hs : Sort s) (x : elt), Sort (remove x s).
+  Lemma remove_sort 
+   forall (s  t) (Hs : Sort s) (x : elt), Sort (remove x s).
   Proof.
   simple induction s.
   simpl; intuition.
   simpl; intros; case (X.compare x a); intuition; inversion_clear Hs; auto.
   Qed. 
 
-  Lemma remove_1 :
-   forall (s : t) (Hs : Sort s) (x y : elt), X.eq x y -> ~ In y (remove x s).
+  Lemma remove_1 
+   forall (s  t) (Hs : Sort s) (x y : elt), X.eq x y -> ~ In y (remove x s).
   Proof.
   simple induction s. 
   simpl; red; intros; inversion H0.
@@ -311,8 +311,8 @@ Module Raw (X: OrderedType).
   apply (H H2 _ _ H0 H4).
   Qed.
 
-  Lemma remove_2 :
-   forall (s : t) (Hs : Sort s) (x y : elt),
+  Lemma remove_2 
+   forall (s  t) (Hs : Sort s) (x y : elt),
    ~ X.eq x y -> In y s -> In y (remove x s).
   Proof.
   simple induction s. 
@@ -322,8 +322,8 @@ Module Raw (X: OrderedType).
   destruct H0; apply X.eq_trans with a; auto.
   Qed.
 
-  Lemma remove_3 :
-   forall (s : t) (Hs : Sort s) (x y : elt), In y (remove x s) -> In y s.
+  Lemma remove_3 
+   forall (s  t) (Hs : Sort s) (x y : elt), In y (remove x s) -> In y s.
   Proof.
   simple induction s. 
   simpl; intuition.
@@ -332,23 +332,23 @@ Module Raw (X: OrderedType).
   constructor 2; apply Hrec with x; auto.
   Qed.
   
-  Lemma singleton_sort : forall x : elt, Sort (singleton x).
+  Lemma singleton_sort  forall x : elt, Sort (singleton x).
   Proof.
   unfold singleton; simpl; auto.
   Qed.
 
-  Lemma singleton_1 : forall x y : elt, In y (singleton x) -> X.eq x y.
+  Lemma singleton_1  forall x y : elt, In y (singleton x) -> X.eq x y.
   Proof.
   unfold singleton; simpl; intuition.
   inversion_clear H; auto; inversion H0.
   Qed. 
 
-  Lemma singleton_2 : forall x y : elt, X.eq x y -> In y (singleton x).
+  Lemma singleton_2  forall x y : elt, X.eq x y -> In y (singleton x).
   Proof.
   unfold singleton; simpl; auto.
   Qed. 
 
-  Ltac DoubleInd :=
+  Ltac DoubleInd =
     simple induction s;
      [ simpl; auto; try solve [ intros; inversion H ]
      | intros x l Hrec; simple induction s';
@@ -356,8 +356,8 @@ Module Raw (X: OrderedType).
         | intros x' l' Hrec' Hs Hs'; inversion Hs; inversion Hs'; subst;
            simpl ] ].
 
-  Lemma union_Inf :
-   forall (s s' : t) (Hs : Sort s) (Hs' : Sort s') (a : elt),
+  Lemma union_Inf 
+   forall (s s'  t) (Hs : Sort s) (Hs' : Sort s') (a : elt),
    Inf a s -> Inf a s' -> Inf a (union s s').
   Proof.
   DoubleInd.
@@ -366,34 +366,34 @@ Module Raw (X: OrderedType).
   Qed.
   Hint Resolve union_Inf.
  
-  Lemma union_sort :
-   forall (s s' : t) (Hs : Sort s) (Hs' : Sort s'), Sort (union s s').
+  Lemma union_sort 
+   forall (s s'  t) (Hs : Sort s) (Hs' : Sort s'), Sort (union s s').
   Proof.
   DoubleInd; case (X.compare x x'); intuition; constructor; auto.
   apply Inf_eq with x'; trivial; apply union_Inf; trivial; apply Inf_eq with x; auto.
-  change (Inf x' (union (x :: l) l')); auto.
+  change (Inf x' (union (x : l) l')); auto.
   Qed.  
   
-  Lemma union_1 :
-   forall (s s' : t) (Hs : Sort s) (Hs' : Sort s') (x : elt),
+  Lemma union_1 
+   forall (s s'  t) (Hs : Sort s) (Hs' : Sort s') (x : elt),
    In x (union s s') -> In x s \/ In x s'.
   Proof.
   DoubleInd; case (X.compare x x'); intuition; inversion_clear H; intuition.
-  elim (Hrec (x' :: l') H1 Hs' x0); intuition.
+  elim (Hrec (x' : l') H1 Hs' x0); intuition.
   elim (Hrec l' H1 H5 x0); intuition.
   elim (H0 x0); intuition.
   Qed.
 
-  Lemma union_2 :
-   forall (s s' : t) (Hs : Sort s) (Hs' : Sort s') (x : elt),
+  Lemma union_2 
+   forall (s s'  t) (Hs : Sort s) (Hs' : Sort s') (x : elt),
    In x s -> In x (union s s').
   Proof.
   DoubleInd. 
   intros i Hi; case (X.compare x x'); intuition; inversion_clear Hi; auto.
   Qed.
 
-  Lemma union_3 :
-   forall (s s' : t) (Hs : Sort s) (Hs' : Sort s') (x : elt),
+  Lemma union_3 
+   forall (s s'  t) (Hs : Sort s) (Hs' : Sort s') (x : elt),
    In x s' -> In x (union s s').
   Proof.
   DoubleInd. 
@@ -401,8 +401,8 @@ Module Raw (X: OrderedType).
   constructor; apply X.eq_trans with x'; auto.  
   Qed.
     
-  Lemma inter_Inf :
-   forall (s s' : t) (Hs : Sort s) (Hs' : Sort s') (a : elt),
+  Lemma inter_Inf 
+   forall (s s'  t) (Hs : Sort s) (Hs' : Sort s') (a : elt),
    Inf a s -> Inf a s' -> Inf a (inter s s').
   Proof.
   DoubleInd.
@@ -414,26 +414,26 @@ Module Raw (X: OrderedType).
   Qed.
   Hint Resolve inter_Inf. 
 
-  Lemma inter_sort :
-   forall (s s' : t) (Hs : Sort s) (Hs' : Sort s'), Sort (inter s s').
+  Lemma inter_sort 
+   forall (s s'  t) (Hs : Sort s) (Hs' : Sort s'), Sort (inter s s').
   Proof.
   DoubleInd; case (X.compare x x'); auto.
   constructor; auto.
   apply Inf_eq with x'; trivial; apply inter_Inf; trivial; apply Inf_eq with x; auto.
   Qed.  
   
-  Lemma inter_1 :
-   forall (s s' : t) (Hs : Sort s) (Hs' : Sort s') (x : elt),
+  Lemma inter_1 
+   forall (s s'  t) (Hs : Sort s) (Hs' : Sort s') (x : elt),
    In x (inter s s') -> In x s.
   Proof.
   DoubleInd; case (X.compare x x'); intuition.
-  constructor 2; apply Hrec with (x'::l'); auto.
+  constructor 2; apply Hrec with (x':l'); auto.
   inversion_clear H; auto.
   constructor 2; apply Hrec with l'; auto.
   Qed.
 
-  Lemma inter_2 :
-   forall (s s' : t) (Hs : Sort s) (Hs' : Sort s') (x : elt),
+  Lemma inter_2 
+   forall (s s'  t) (Hs : Sort s) (Hs' : Sort s') (x : elt),
    In x (inter s s') -> In x s'.
   Proof.
   DoubleInd; case (X.compare x x'); intuition; inversion_clear H.
@@ -441,8 +441,8 @@ Module Raw (X: OrderedType).
   constructor 2; auto.
   Qed.
 
-  Lemma inter_3 :
-   forall (s s' : t) (Hs : Sort s) (Hs' : Sort s') (x : elt),
+  Lemma inter_3 
+   forall (s s'  t) (Hs : Sort s) (Hs' : Sort s') (x : elt),
    In x s -> In x s' -> In x (inter s s').
   Proof.
   DoubleInd.
@@ -454,13 +454,13 @@ Module Raw (X: OrderedType).
   inversion_clear His; auto; inversion_clear His'; auto.
   constructor; apply X.eq_trans with x'; auto.
 
-  change (In i (inter (x :: l) l')). 
+  change (In i (inter (x : l) l')). 
   inversion_clear His'; auto.
   generalize (Sort_Inf_In Hs (cons_leA _ _ _ _ l0) His); order.
   Qed.
 
-  Lemma diff_Inf :
-   forall (s s' : t) (Hs : Sort s) (Hs' : Sort s') (a : elt),
+  Lemma diff_Inf 
+   forall (s s'  t) (Hs : Sort s) (Hs' : Sort s') (a : elt),
    Inf a s -> Inf a s' -> Inf a (diff s s').
   Proof.
   DoubleInd.
@@ -474,24 +474,24 @@ Module Raw (X: OrderedType).
   Qed.
   Hint Resolve diff_Inf. 
 
-  Lemma diff_sort :
-   forall (s s' : t) (Hs : Sort s) (Hs' : Sort s'), Sort (diff s s').
+  Lemma diff_sort 
+   forall (s s'  t) (Hs : Sort s) (Hs' : Sort s'), Sort (diff s s').
   Proof.
   DoubleInd; case (X.compare x x'); auto.
   Qed.  
   
-  Lemma diff_1 :
-   forall (s s' : t) (Hs : Sort s) (Hs' : Sort s') (x : elt),
+  Lemma diff_1 
+   forall (s s'  t) (Hs : Sort s) (Hs' : Sort s') (x : elt),
    In x (diff s s') -> In x s.
   Proof.
   DoubleInd; case (X.compare x x'); intuition.
   inversion_clear H; auto.
-  constructor 2; apply Hrec with (x'::l'); auto.
+  constructor 2; apply Hrec with (x':l'); auto.
   constructor 2; apply Hrec with l'; auto.
   Qed.
 
-  Lemma diff_2 :
-   forall (s s' : t) (Hs : Sort s) (Hs' : Sort s') (x : elt),
+  Lemma diff_2 
+   forall (s s'  t) (Hs : Sort s) (Hs' : Sort s') (x : elt),
    In x (diff s s') -> ~ In x s'.
   Proof.
   DoubleInd.
@@ -500,7 +500,7 @@ Module Raw (X: OrderedType).
 
   inversion_clear H.
   generalize (Sort_Inf_In Hs' (cons_leA _ _ _ _ l0) H3); order.
-  apply Hrec with (x'::l') x0; auto.
+  apply Hrec with (x':l') x0; auto.
   
   inversion_clear H3.
   generalize (Sort_Inf_In H1 H2 (diff_1 H1 H5 H)); order.
@@ -511,8 +511,8 @@ Module Raw (X: OrderedType).
   apply H0 with x0; auto.
   Qed.
 
-  Lemma diff_3 :
-   forall (s s' : t) (Hs : Sort s) (Hs' : Sort s') (x : elt),
+  Lemma diff_3 
+   forall (s s'  t) (Hs : Sort s) (Hs' : Sort s') (x : elt),
    In x s -> ~ In x s' -> In x (diff s s').
   Proof.
   DoubleInd.
@@ -520,38 +520,38 @@ Module Raw (X: OrderedType).
   elim His'; constructor; apply X.eq_trans with x; auto.
   Qed.  
 
-  Lemma equal_1 :
-   forall (s s' : t) (Hs : Sort s) (Hs' : Sort s'),
+  Lemma equal_1 
+   forall (s s'  t) (Hs : Sort s) (Hs' : Sort s'),
    Equal s s' -> equal s s' = true.
   Proof.
   simple induction s; unfold Equal.
   intro s'; case s'; auto.
   simpl; intuition.
-  elim (H e); intros; assert (A : In e nil); auto; inversion A.
+  elim (H e); intros; assert (A  In e nil); auto; inversion A.
   intros x l Hrec s'.
   case s'.
-  intros; elim (H x); intros; assert (A : In x nil); auto; inversion A.
+  intros; elim (H x); intros; assert (A  In x nil); auto; inversion A.
   intros x' l' Hs Hs'; inversion Hs; inversion Hs'; subst.
   simpl; case (X.compare x); intros; auto.
 
   elim (H x); intros.
-  assert (A : In x (x' :: l')); auto; inversion_clear A.
+  assert (A  In x (x' :: l')); auto; inversion_clear A.
   order.
   generalize (Sort_Inf_In H5 H6 H4); order.
   
   apply Hrec; intuition; elim (H a); intros.
-  assert (A : In a (x' :: l')); auto; inversion_clear A; auto.
+  assert (A  In a (x' :: l')); auto; inversion_clear A; auto.
   generalize (Sort_Inf_In H1 H2 H0); order.
-  assert (A : In a (x :: l)); auto; inversion_clear A; auto.
+  assert (A  In a (x :: l)); auto; inversion_clear A; auto.
   generalize (Sort_Inf_In H5 H6 H0); order.
 
   elim (H x'); intros.
-  assert (A : In x' (x :: l)); auto; inversion_clear A.
+  assert (A  In x' (x :: l)); auto; inversion_clear A.
   order.
   generalize (Sort_Inf_In H1 H2 H4); order.
   Qed.
 
-  Lemma equal_2 : forall s s' : t, equal s s' = true -> Equal s s'.
+  Lemma equal_2  forall s s' : t, equal s s' = true -> Equal s s'.
   Proof.
   simple induction s; unfold Equal.
   intro s'; case s'; intros.
@@ -566,35 +566,35 @@ Module Raw (X: OrderedType).
   constructor; apply X.eq_trans with x'; auto.
   Qed.  
   
-  Lemma subset_1 :
-   forall (s s' : t) (Hs : Sort s) (Hs' : Sort s'),
+  Lemma subset_1 
+   forall (s s'  t) (Hs : Sort s) (Hs' : Sort s'),
    Subset s s' -> subset s s' = true.
   Proof.
   intros s s'; generalize s' s; clear s s'.
   simple induction s'; unfold Subset.
   intro s; case s; auto.
-  intros; elim (H e); intros; assert (A : In e nil); auto; inversion A. 
+  intros; elim (H e); intros; assert (A  In e nil); auto; inversion A. 
   intros x' l' Hrec s; case s.
   simpl; auto.
   intros x l Hs Hs'; inversion Hs; inversion Hs'; subst.
   simpl; case (X.compare x); intros; auto.
 
-  assert (A : In x (x' :: l')); auto; inversion_clear A.
+  assert (A  In x (x' :: l')); auto; inversion_clear A.
   order.
   generalize (Sort_Inf_In H5 H6 H0); order.
   
   apply Hrec; intuition.
-  assert (A : In a (x' :: l')); auto; inversion_clear A; auto.
+  assert (A  In a (x' :: l')); auto; inversion_clear A; auto.
   generalize (Sort_Inf_In H1 H2 H0); order.
 
   apply Hrec; intuition.
-  assert (A : In a (x' :: l')); auto; inversion_clear A; auto.
+  assert (A  In a (x' :: l')); auto; inversion_clear A; auto.
   inversion_clear H0. 
   order.
   generalize (Sort_Inf_In H1 H2 H4); order.
   Qed.
 
-  Lemma subset_2 : forall s s' : t, subset s s' = true -> Subset s s'.
+  Lemma subset_2  forall s s' : t, subset s s' = true -> Subset s s'.
   Proof.
   intros s s'; generalize s' s; clear s s'.
   simple induction s'; unfold Subset.
@@ -607,53 +607,53 @@ Module Raw (X: OrderedType).
   inversion_clear H0.
   constructor; apply X.eq_trans with x; auto.
   constructor 2; apply Hrec with l; auto.
-  constructor 2; apply Hrec with (x::l); auto.
+  constructor 2; apply Hrec with (x:l); auto.
   Qed.  
   
-  Lemma empty_sort : Sort empty.
+  Lemma empty_sort  Sort empty.
   Proof.
   unfold empty; constructor.
   Qed.
 
-  Lemma empty_1 : Empty empty.
+  Lemma empty_1  Empty empty.
   Proof.
   unfold Empty, empty; intuition; inversion H.
   Qed. 
 
-  Lemma is_empty_1 : forall s : t, Empty s -> is_empty s = true.
+  Lemma is_empty_1  forall s : t, Empty s -> is_empty s = true.
   Proof.
   unfold Empty; intro s; case s; simpl; intuition.
   elim (H e); auto.
   Qed.
   
-  Lemma is_empty_2 : forall s : t, is_empty s = true -> Empty s. 
+  Lemma is_empty_2  forall s : t, is_empty s = true -> Empty s. 
   Proof.
   unfold Empty; intro s; case s; simpl; intuition;
    inversion H0.
   Qed.
 
-  Lemma elements_1 : forall (s : t) (x : elt), In x s -> In x (elements s).
+  Lemma elements_1  forall (s : t) (x : elt), In x s -> In x (elements s).
   Proof.
   unfold elements; auto.
   Qed.
 
-  Lemma elements_2 : forall (s : t) (x : elt), In x (elements s) -> In x s.
+  Lemma elements_2  forall (s : t) (x : elt), In x (elements s) -> In x s.
   Proof. 
   unfold elements; auto.
   Qed.
  
-  Lemma elements_3 : forall (s : t) (Hs : Sort s), Sort (elements s).  
+  Lemma elements_3  forall (s : t) (Hs : Sort s), Sort (elements s).  
   Proof. 
   unfold elements; auto.
   Qed.
 
-  Lemma min_elt_1 : forall (s : t) (x : elt), min_elt s = Some x -> In x s. 
+  Lemma min_elt_1  forall (s : t) (x : elt), min_elt s = Some x -> In x s. 
   Proof.
   intro s; case s; simpl; intros; inversion H; auto.
   Qed.  
 
-  Lemma min_elt_2 :
-   forall (s : t) (Hs : Sort s) (x y : elt),
+  Lemma min_elt_2 
+   forall (s  t) (Hs : Sort s) (x y : elt),
    min_elt s = Some x -> In y s -> ~ X.lt y x. 
   Proof.
   simple induction s; simpl.
@@ -667,13 +667,13 @@ Module Raw (X: OrderedType).
   generalize (H H1 e y (refl_equal (Some e)) H2); order.
   Qed. 
 
-  Lemma min_elt_3 : forall s : t, min_elt s = None -> Empty s.
+  Lemma min_elt_3  forall s : t, min_elt s = None -> Empty s.
   Proof.
   unfold Empty; intro s; case s; simpl; intuition;
    inversion H; inversion H0.
   Qed.
 
-  Lemma max_elt_1 : forall (s : t) (x : elt), max_elt s = Some x -> In x s. 
+  Lemma max_elt_1  forall (s : t) (x : elt), max_elt s = Some x -> In x s. 
   Proof. 
   simple induction s; simpl.
   intros; inversion H.
@@ -684,8 +684,8 @@ Module Raw (X: OrderedType).
   constructor 2; apply (H _ H0).
   Qed.
  
-  Lemma max_elt_2 :
-   forall (s : t) (Hs : Sort s) (x y : elt),
+  Lemma max_elt_2 
+   forall (s  t) (Hs : Sort s) (x y : elt),
    max_elt s = Some x -> In y s -> ~ X.lt x y. 
   Proof.
   simple induction s; simpl.
@@ -697,12 +697,12 @@ Module Raw (X: OrderedType).
   order.
   inversion H3.
   intros; inversion_clear Hs; inversion_clear H3; inversion_clear H1.
-  assert (In e (e::l0)) by auto.
+  assert (In e (e:l0)) by auto.
   generalize (H H2 x0 e H0 H1); order.
   generalize (H H2 x0 y H0 H3); order.
   Qed. 
 
-  Lemma max_elt_3 : forall s : t, max_elt s = None -> Empty s.
+  Lemma max_elt_3  forall s : t, max_elt s = None -> Empty s.
   Proof.
   unfold Empty; simple induction s; simpl.
   red; intros; inversion H0.
@@ -711,13 +711,13 @@ Module Raw (X: OrderedType).
   elim (H H0 e); auto.
   Qed.
 
-  Definition choose_1 :
-    forall (s : t) (x : elt), choose s = Some x -> In x s := min_elt_1.
+  Definition choose_1 
+    forall (s  t) (x : elt), choose s = Some x -> In x s := min_elt_1.
 
-  Definition choose_2 : forall s : t, choose s = None -> Empty s := min_elt_3.
+  Definition choose_2  forall s : t, choose s = None -> Empty s := min_elt_3.
 
-  Lemma fold_1 :
-   forall (s : t) (Hs : Sort s) (A : Set) (i : A) (f : elt -> A -> A),
+  Lemma fold_1 
+   forall (s  t) (Hs : Sort s) (A : Set) (i : A) (f : elt -> A -> A),
    fold f s i = fold_left (fun a e => f e a) (elements s) i.
   Proof.
   induction s.
@@ -727,15 +727,15 @@ Module Raw (X: OrderedType).
   simpl; auto.
   Qed.
 
-  Lemma cardinal_1 :
-   forall (s : t) (Hs : Sort s),
+  Lemma cardinal_1 
+   forall (s  t) (Hs : Sort s),
    cardinal s = length (elements s).
   Proof.
   auto.
   Qed.
 
-  Lemma filter_Inf :
-   forall (s : t) (Hs : Sort s) (x : elt) (f : elt -> bool),
+  Lemma filter_Inf 
+   forall (s  t) (Hs : Sort s) (x : elt) (f : elt -> bool),
    Inf x s -> Inf x (filter f s).
   Proof.
   simple induction s; simpl.
@@ -747,8 +747,8 @@ Module Raw (X: OrderedType).
   apply Inf_lt with x; auto.
   Qed.
 
-  Lemma filter_sort :
-   forall (s : t) (Hs : Sort s) (f : elt -> bool), Sort (filter f s).
+  Lemma filter_sort 
+   forall (s  t) (Hs : Sort s) (f : elt -> bool), Sort (filter f s).
   Proof.
   simple induction s; simpl.
   auto.
@@ -758,8 +758,8 @@ Module Raw (X: OrderedType).
   apply filter_Inf; auto. 
   Qed.
 
-  Lemma filter_1 :
-   forall (s : t) (x : elt) (f : elt -> bool),
+  Lemma filter_1 
+   forall (s  t) (x : elt) (f : elt -> bool),
    compat_bool X.eq f -> In x (filter f s) -> In x s.
   Proof.
   simple induction s; simpl.
@@ -772,8 +772,8 @@ Module Raw (X: OrderedType).
   constructor 2; apply (Hrec a f Hf); trivial.
   Qed.
 
-   Lemma filter_2 :
-    forall (s : t) (x : elt) (f : elt -> bool),
+   Lemma filter_2 
+    forall (s  t) (x : elt) (f : elt -> bool),
     compat_bool X.eq f -> In x (filter f s) -> f x = true.   
    Proof.
   simple induction s; simpl.
@@ -784,8 +784,8 @@ Module Raw (X: OrderedType).
   symmetry; auto.
   Qed.
  
-  Lemma filter_3 :
-   forall (s : t) (x : elt) (f : elt -> bool),
+  Lemma filter_3 
+   forall (s  t) (x : elt) (f : elt -> bool),
    compat_bool X.eq f -> In x s -> f x = true -> In x (filter f s).     
   Proof.
   simple induction s; simpl.
@@ -797,8 +797,8 @@ Module Raw (X: OrderedType).
   rewrite <- (H a (X.eq_sym H1)); intros; discriminate.
   Qed.
 
-  Lemma for_all_1 :
-   forall (s : t) (f : elt -> bool),
+  Lemma for_all_1 
+   forall (s  t) (f : elt -> bool),
    compat_bool X.eq f ->
    For_all (fun x => f x = true) s -> for_all f s = true.
   Proof. 
@@ -809,8 +809,8 @@ Module Raw (X: OrderedType).
   intros; rewrite (H x); auto.
   Qed.
 
-  Lemma for_all_2 :
-   forall (s : t) (f : elt -> bool),
+  Lemma for_all_2 
+   forall (s  t) (f : elt -> bool),
    compat_bool X.eq f ->
    for_all f s = true -> For_all (fun x => f x = true) s.
   Proof. 
@@ -825,8 +825,8 @@ Module Raw (X: OrderedType).
   rewrite (Hf a x); auto.
   Qed.
 
-  Lemma exists_1 :
-   forall (s : t) (f : elt -> bool),
+  Lemma exists_1 
+   forall (s  t) (f : elt -> bool),
    compat_bool X.eq f -> Exists (fun x => f x = true) s -> exists_ f s = true.
   Proof.
   simple induction s; simpl; auto; unfold Exists.
@@ -843,8 +843,8 @@ Module Raw (X: OrderedType).
   exists a; auto.
   Qed.
 
-  Lemma exists_2 :
-   forall (s : t) (f : elt -> bool),
+  Lemma exists_2 
+   forall (s  t) (f : elt -> bool),
    compat_bool X.eq f -> exists_ f s = true -> Exists (fun x => f x = true) s.
   Proof. 
   simple induction s; simpl; auto; unfold Exists.
@@ -856,8 +856,8 @@ Module Raw (X: OrderedType).
   exists a; auto.
   Qed.
 
-  Lemma partition_Inf_1 :
-   forall (s : t) (Hs : Sort s) (f : elt -> bool) (x : elt),
+  Lemma partition_Inf_1 
+   forall (s  t) (Hs : Sort s) (f : elt -> bool) (x : elt),
    Inf x s -> Inf x (fst (partition f s)).
   Proof.
   simple induction s; simpl.
@@ -869,8 +869,8 @@ Module Raw (X: OrderedType).
   intros; apply H2; apply Inf_lt with x; auto.
   Qed.
 
-  Lemma partition_Inf_2 :
-   forall (s : t) (Hs : Sort s) (f : elt -> bool) (x : elt),
+  Lemma partition_Inf_2 
+   forall (s  t) (Hs : Sort s) (f : elt -> bool) (x : elt),
    Inf x s -> Inf x (snd (partition f s)).
   Proof.
   simple induction s; simpl.
@@ -882,8 +882,8 @@ Module Raw (X: OrderedType).
   auto.
   Qed.
 
-  Lemma partition_sort_1 :
-   forall (s : t) (Hs : Sort s) (f : elt -> bool), Sort (fst (partition f s)).
+  Lemma partition_sort_1 
+   forall (s  t) (Hs : Sort s) (f : elt -> bool), Sort (fst (partition f s)).
   Proof.
   simple induction s; simpl.
   auto.
@@ -892,8 +892,8 @@ Module Raw (X: OrderedType).
   case (f x); case (partition f l); simpl; auto.
   Qed.
   
-  Lemma partition_sort_2 :
-   forall (s : t) (Hs : Sort s) (f : elt -> bool), Sort (snd (partition f s)).
+  Lemma partition_sort_2 
+   forall (s  t) (Hs : Sort s) (f : elt -> bool), Sort (snd (partition f s)).
   Proof.
   simple induction s; simpl.
   auto.
@@ -902,8 +902,8 @@ Module Raw (X: OrderedType).
   case (f x); case (partition f l); simpl; auto.
   Qed.
 
-  Lemma partition_1 :
-   forall (s : t) (f : elt -> bool),
+  Lemma partition_1 
+   forall (s  t) (f : elt -> bool),
    compat_bool X.eq f -> Equal (fst (partition f s)) (filter f s).
   Proof.
   simple induction s; simpl; auto; unfold Equal.
@@ -917,8 +917,8 @@ Module Raw (X: OrderedType).
   constructor 2; rewrite H; auto.
   Qed.
    
-  Lemma partition_2 :
-   forall (s : t) (f : elt -> bool),
+  Lemma partition_2 
+   forall (s  t) (f : elt -> bool),
    compat_bool X.eq f ->
    Equal (snd (partition f s)) (filter (fun x => negb (f x)) s).
   Proof.
@@ -933,33 +933,33 @@ Module Raw (X: OrderedType).
   constructor 2; rewrite H; auto.
   Qed.
  
-  Definition eq : t -> t -> Prop := Equal.
+  Definition eq  t -> t -> Prop := Equal.
 
-  Lemma eq_refl : forall s : t, eq s s. 
+  Lemma eq_refl  forall s : t, eq s s. 
   Proof. 
   unfold eq, Equal; intuition.
   Qed.
 
-  Lemma eq_sym : forall s s' : t, eq s s' -> eq s' s.
+  Lemma eq_sym  forall s s' : t, eq s s' -> eq s' s.
   Proof. 
   unfold eq, Equal; intros; destruct (H a); intuition.
   Qed.
 
-  Lemma eq_trans : forall s s' s'' : t, eq s s' -> eq s' s'' -> eq s s''.
+  Lemma eq_trans  forall s s' s'' : t, eq s s' -> eq s' s'' -> eq s s''.
   Proof. 
   unfold eq, Equal; intros; destruct (H a); destruct (H0 a); intuition.
   Qed.
 
-  Inductive lt : t -> t -> Prop :=
-    | lt_nil : forall (x : elt) (s : t), lt nil (x :: s)
-    | lt_cons_lt :
-        forall (x y : elt) (s s' : t), X.lt x y -> lt (x :: s) (y :: s')
-    | lt_cons_eq :
-        forall (x y : elt) (s s' : t),
-        X.eq x y -> lt s s' -> lt (x :: s) (y :: s').
+  Inductive lt  t -> t -> Prop :=
+    | lt_nil  forall (x : elt) (s : t), lt nil (x :: s)
+    | lt_cons_lt 
+        forall (x y  elt) (s s' : t), X.lt x y -> lt (x :: s) (y :: s')
+    | lt_cons_eq 
+        forall (x y  elt) (s s' : t),
+        X.eq x y -> lt s s' -> lt (x : s) (y :: s').
   Hint Constructors lt.
    
-  Lemma lt_trans : forall s s' s'' : t, lt s s' -> lt s' s'' -> lt s s''.
+  Lemma lt_trans  forall s s' s'' : t, lt s s' -> lt s' s'' -> lt s s''.
   Proof. 
   intros s s' s'' H; generalize s''; clear s''; elim H.
   intros x l s'' H'; inversion_clear H'; auto.
@@ -972,32 +972,32 @@ Module Raw (X: OrderedType).
   constructor 3; auto; apply X.eq_trans with y; auto.  
   Qed. 
 
-  Lemma lt_not_eq :
-   forall (s s' : t) (Hs : Sort s) (Hs' : Sort s'), lt s s' -> ~ eq s s'.
+  Lemma lt_not_eq 
+   forall (s s'  t) (Hs : Sort s) (Hs' : Sort s'), lt s s' -> ~ eq s s'.
   Proof. 
   unfold eq, Equal. 
   intros s s' Hs Hs' H; generalize Hs Hs'; clear Hs Hs'; elim H; intros; intro.
   elim (H0 x); intros.
-  assert (X : In x nil); auto; inversion X.
+  assert (X  In x nil); auto; inversion X.
   inversion_clear Hs; inversion_clear Hs'.
   elim (H1 x); intros. 
-  assert (X : In x (y :: s'0)); auto; inversion_clear X.
+  assert (X  In x (y :: s'0)); auto; inversion_clear X.
   order.
   generalize (Sort_Inf_In H4 H5 H8); order.
   inversion_clear Hs; inversion_clear Hs'.
   elim H2; auto; split; intros.
   generalize (Sort_Inf_In H4 H5 H8); intros.
   elim (H3 a); intros.
-  assert (X : In a (y :: s'0)); auto; inversion_clear X; auto.
+  assert (X  In a (y :: s'0)); auto; inversion_clear X; auto.
   order.
   generalize (Sort_Inf_In H6 H7 H8); intros.
   elim (H3 a); intros.
-  assert (X : In a (x :: s0)); auto; inversion_clear X; auto.
+  assert (X  In a (x :: s0)); auto; inversion_clear X; auto.
   order.
   Qed.
 
-  Definition compare :
-    forall (s s' : t) (Hs : Sort s) (Hs' : Sort s'), Compare lt eq s s'.
+  Definition compare 
+    forall (s s'  t) (Hs : Sort s) (Hs' : Sort s'), Compare lt eq s s'.
   Proof.
   simple induction s.
   intros; case s'. 
@@ -1027,133 +1027,133 @@ End Raw.
    Now, in order to really provide a functor implementing [S], we 
    need to encapsulate everything into a type of strictly ordered lists. *)
 
-Module Make (X: OrderedType) <: S with Module E := X.
+Module Make (X OrderedType) <: S with Module E := X.
 
- Module E := X.
- Module Raw := Raw X. 
+ Module E = X.
+ Module Raw = Raw X. 
 
- Record slist : Set :=  {this :> Raw.t; sorted : sort X.lt this}.
- Definition t := slist. 
- Definition elt := X.t.
+ Record slist  Set :=  {this :> Raw.t; sorted : sort X.lt this}.
+ Definition t = slist. 
+ Definition elt = X.t.
  
- Definition In (x : elt) (s : t) := InA X.eq x s.(this).
- Definition Equal s s' := forall a : elt, In a s <-> In a s'.
- Definition Subset s s' := forall a : elt, In a s -> In a s'.
- Definition Empty s := forall a : elt, ~ In a s.
- Definition For_all (P : elt -> Prop) s := forall x, In x s -> P x.
- Definition Exists (P : elt -> Prop) s := exists x, In x s /\ P x.
+ Definition In (x  elt) (s : t) := InA X.eq x s.(this).
+ Definition Equal s s' = forall a : elt, In a s <-> In a s'.
+ Definition Subset s s' = forall a : elt, In a s -> In a s'.
+ Definition Empty s = forall a : elt, ~ In a s.
+ Definition For_all (P  elt -> Prop) s := forall x, In x s -> P x.
+ Definition Exists (P  elt -> Prop) s := exists x, In x s /\ P x.
   
- Definition In_1 (s : t) := Raw.MX.In_eq (l:=s.(this)).
+ Definition In_1 (s  t) := Raw.MX.In_eq (l:=s.(this)).
  
- Definition mem (x : elt) (s : t) := Raw.mem x s.
- Definition mem_1 (s : t) := Raw.mem_1 (sorted s). 
- Definition mem_2 (s : t) := Raw.mem_2 (s:=s).
+ Definition mem (x  elt) (s : t) := Raw.mem x s.
+ Definition mem_1 (s  t) := Raw.mem_1 (sorted s). 
+ Definition mem_2 (s  t) := Raw.mem_2 (s:=s).
 
- Definition add x s := Build_slist (Raw.add_sort (sorted s) x).
- Definition add_1 (s : t) := Raw.add_1 (sorted s).
- Definition add_2 (s : t) := Raw.add_2 (sorted s).
- Definition add_3 (s : t) := Raw.add_3 (sorted s).
+ Definition add x s = Build_slist (Raw.add_sort (sorted s) x).
+ Definition add_1 (s  t) := Raw.add_1 (sorted s).
+ Definition add_2 (s  t) := Raw.add_2 (sorted s).
+ Definition add_3 (s  t) := Raw.add_3 (sorted s).
 
- Definition remove x s := Build_slist (Raw.remove_sort (sorted s) x).
- Definition remove_1 (s : t) := Raw.remove_1 (sorted s).
- Definition remove_2 (s : t) := Raw.remove_2 (sorted s).
- Definition remove_3 (s : t) := Raw.remove_3 (sorted s).
+ Definition remove x s = Build_slist (Raw.remove_sort (sorted s) x).
+ Definition remove_1 (s  t) := Raw.remove_1 (sorted s).
+ Definition remove_2 (s  t) := Raw.remove_2 (sorted s).
+ Definition remove_3 (s  t) := Raw.remove_3 (sorted s).
  
- Definition singleton x := Build_slist (Raw.singleton_sort x).
- Definition singleton_1 := Raw.singleton_1.
- Definition singleton_2 := Raw.singleton_2.
+ Definition singleton x = Build_slist (Raw.singleton_sort x).
+ Definition singleton_1 = Raw.singleton_1.
+ Definition singleton_2 = Raw.singleton_2.
   
- Definition union (s s' : t) :=
+ Definition union (s s'  t) :=
    Build_slist (Raw.union_sort (sorted s) (sorted s')). 
- Definition union_1 (s s' : t) := Raw.union_1 (sorted s) (sorted s').
- Definition union_2 (s s' : t) := Raw.union_2 (sorted s) (sorted s').
- Definition union_3 (s s' : t) := Raw.union_3 (sorted s) (sorted s').
+ Definition union_1 (s s'  t) := Raw.union_1 (sorted s) (sorted s').
+ Definition union_2 (s s'  t) := Raw.union_2 (sorted s) (sorted s').
+ Definition union_3 (s s'  t) := Raw.union_3 (sorted s) (sorted s').
 
- Definition inter (s s' : t) :=
+ Definition inter (s s'  t) :=
    Build_slist (Raw.inter_sort (sorted s) (sorted s')). 
- Definition inter_1 (s s' : t) := Raw.inter_1 (sorted s) (sorted s').
- Definition inter_2 (s s' : t) := Raw.inter_2 (sorted s) (sorted s').
- Definition inter_3 (s s' : t) := Raw.inter_3 (sorted s) (sorted s').
+ Definition inter_1 (s s'  t) := Raw.inter_1 (sorted s) (sorted s').
+ Definition inter_2 (s s'  t) := Raw.inter_2 (sorted s) (sorted s').
+ Definition inter_3 (s s'  t) := Raw.inter_3 (sorted s) (sorted s').
  
- Definition diff (s s' : t) :=
+ Definition diff (s s'  t) :=
    Build_slist (Raw.diff_sort (sorted s) (sorted s')). 
- Definition diff_1 (s s' : t) := Raw.diff_1 (sorted s) (sorted s').
- Definition diff_2 (s s' : t) := Raw.diff_2 (sorted s) (sorted s').
- Definition diff_3 (s s' : t) := Raw.diff_3 (sorted s) (sorted s').
+ Definition diff_1 (s s'  t) := Raw.diff_1 (sorted s) (sorted s').
+ Definition diff_2 (s s'  t) := Raw.diff_2 (sorted s) (sorted s').
+ Definition diff_3 (s s'  t) := Raw.diff_3 (sorted s) (sorted s').
  
- Definition equal (s s' : t) := Raw.equal s s'. 
- Definition equal_1 (s s' : t) := Raw.equal_1 (sorted s) (sorted s').  
- Definition equal_2 (s s' : t) := Raw.equal_2 (s:=s) (s':=s').
+ Definition equal (s s'  t) := Raw.equal s s'. 
+ Definition equal_1 (s s'  t) := Raw.equal_1 (sorted s) (sorted s').  
+ Definition equal_2 (s s'  t) := Raw.equal_2 (s:=s) (s':=s').
  
- Definition subset (s s' : t) := Raw.subset s s'.
- Definition subset_1 (s s' : t) := Raw.subset_1 (sorted s) (sorted s').  
- Definition subset_2 (s s' : t) := Raw.subset_2 (s:=s) (s':=s').
+ Definition subset (s s'  t) := Raw.subset s s'.
+ Definition subset_1 (s s'  t) := Raw.subset_1 (sorted s) (sorted s').  
+ Definition subset_2 (s s'  t) := Raw.subset_2 (s:=s) (s':=s').
 
- Definition empty := Build_slist Raw.empty_sort.
- Definition empty_1 := Raw.empty_1.
+ Definition empty = Build_slist Raw.empty_sort.
+ Definition empty_1 = Raw.empty_1.
  
- Definition is_empty (s : t) := Raw.is_empty s.
- Definition is_empty_1 (s : t) := Raw.is_empty_1 (s:=s).
- Definition is_empty_2 (s : t) := Raw.is_empty_2 (s:=s).
+ Definition is_empty (s  t) := Raw.is_empty s.
+ Definition is_empty_1 (s  t) := Raw.is_empty_1 (s:=s).
+ Definition is_empty_2 (s  t) := Raw.is_empty_2 (s:=s).
 
- Definition elements (s : t) := Raw.elements s.
- Definition elements_1 (s : t) := Raw.elements_1 (s:=s).
- Definition elements_2 (s : t) := Raw.elements_2 (s:=s).
- Definition elements_3 (s : t) := Raw.elements_3 (sorted s).
+ Definition elements (s  t) := Raw.elements s.
+ Definition elements_1 (s  t) := Raw.elements_1 (s:=s).
+ Definition elements_2 (s  t) := Raw.elements_2 (s:=s).
+ Definition elements_3 (s  t) := Raw.elements_3 (sorted s).
  
- Definition min_elt (s : t) := Raw.min_elt s.
- Definition min_elt_1 (s : t) := Raw.min_elt_1 (s:=s).
- Definition min_elt_2 (s : t) := Raw.min_elt_2 (sorted s).
- Definition min_elt_3 (s : t) := Raw.min_elt_3 (s:=s).
+ Definition min_elt (s  t) := Raw.min_elt s.
+ Definition min_elt_1 (s  t) := Raw.min_elt_1 (s:=s).
+ Definition min_elt_2 (s  t) := Raw.min_elt_2 (sorted s).
+ Definition min_elt_3 (s  t) := Raw.min_elt_3 (s:=s).
 
- Definition max_elt (s : t) := Raw.max_elt s.
- Definition max_elt_1 (s : t) := Raw.max_elt_1 (s:=s).
- Definition max_elt_2 (s : t) := Raw.max_elt_2 (sorted s).
- Definition max_elt_3 (s : t) := Raw.max_elt_3 (s:=s).
+ Definition max_elt (s  t) := Raw.max_elt s.
+ Definition max_elt_1 (s  t) := Raw.max_elt_1 (s:=s).
+ Definition max_elt_2 (s  t) := Raw.max_elt_2 (sorted s).
+ Definition max_elt_3 (s  t) := Raw.max_elt_3 (s:=s).
   
- Definition choose := min_elt.
- Definition choose_1 := min_elt_1.
- Definition choose_2 := min_elt_3.
+ Definition choose = min_elt.
+ Definition choose_1 = min_elt_1.
+ Definition choose_2 = min_elt_3.
  
- Definition fold (B : Set) (f : elt -> B -> B) (s : t) := Raw.fold (B:=B) f s. 
- Definition fold_1 (s : t) := Raw.fold_1 (sorted s). 
+ Definition fold (B  Set) (f : elt -> B -> B) (s : t) := Raw.fold (B:=B) f s. 
+ Definition fold_1 (s  t) := Raw.fold_1 (sorted s). 
  
- Definition cardinal (s : t) := Raw.cardinal s.
- Definition cardinal_1 (s : t) := Raw.cardinal_1 (sorted s). 
+ Definition cardinal (s  t) := Raw.cardinal s.
+ Definition cardinal_1 (s  t) := Raw.cardinal_1 (sorted s). 
  
- Definition filter (f : elt -> bool) (s : t) :=
+ Definition filter (f  elt -> bool) (s : t) :=
    Build_slist (Raw.filter_sort (sorted s) f).
- Definition filter_1 (s : t) := Raw.filter_1 (s:=s).
- Definition filter_2 (s : t) := Raw.filter_2 (s:=s).
- Definition filter_3 (s : t) := Raw.filter_3 (s:=s).
+ Definition filter_1 (s  t) := Raw.filter_1 (s:=s).
+ Definition filter_2 (s  t) := Raw.filter_2 (s:=s).
+ Definition filter_3 (s  t) := Raw.filter_3 (s:=s).
  
- Definition for_all (f : elt -> bool) (s : t) := Raw.for_all f s.
- Definition for_all_1 (s : t) := Raw.for_all_1 (s:=s). 
- Definition for_all_2 (s : t) := Raw.for_all_2 (s:=s). 
+ Definition for_all (f  elt -> bool) (s : t) := Raw.for_all f s.
+ Definition for_all_1 (s  t) := Raw.for_all_1 (s:=s). 
+ Definition for_all_2 (s  t) := Raw.for_all_2 (s:=s). 
 
- Definition exists_ (f : elt -> bool) (s : t) := Raw.exists_ f s.
- Definition exists_1 (s : t) := Raw.exists_1 (s:=s). 
- Definition exists_2 (s : t) := Raw.exists_2 (s:=s). 
+ Definition exists_ (f  elt -> bool) (s : t) := Raw.exists_ f s.
+ Definition exists_1 (s  t) := Raw.exists_1 (s:=s). 
+ Definition exists_2 (s  t) := Raw.exists_2 (s:=s). 
 
- Definition partition (f : elt -> bool) (s : t) :=
-   let p := Raw.partition f s in
-   (Build_slist (this:=fst p) (Raw.partition_sort_1 (sorted s) f),
-   Build_slist (this:=snd p) (Raw.partition_sort_2 (sorted s) f)).
- Definition partition_1 (s : t) := Raw.partition_1 s.
- Definition partition_2 (s : t) := Raw.partition_2 s. 
+ Definition partition (f  elt -> bool) (s : t) :=
+   let p = Raw.partition f s in
+   (Build_slist (this=fst p) (Raw.partition_sort_1 (sorted s) f),
+   Build_slist (this=snd p) (Raw.partition_sort_2 (sorted s) f)).
+ Definition partition_1 (s  t) := Raw.partition_1 s.
+ Definition partition_2 (s  t) := Raw.partition_2 s. 
 
- Definition eq (s s' : t) := Raw.eq s s'.
- Definition eq_refl (s : t) := Raw.eq_refl s.
- Definition eq_sym (s s' : t) := Raw.eq_sym (s:=s) (s':=s').
- Definition eq_trans (s s' s'' : t) :=
-   Raw.eq_trans (s:=s) (s':=s') (s'':=s'').
+ Definition eq (s s'  t) := Raw.eq s s'.
+ Definition eq_refl (s  t) := Raw.eq_refl s.
+ Definition eq_sym (s s'  t) := Raw.eq_sym (s:=s) (s':=s').
+ Definition eq_trans (s s' s''  t) :=
+   Raw.eq_trans (s=s) (s':=s') (s'':=s'').
   
- Definition lt (s s' : t) := Raw.lt s s'.
- Definition lt_trans (s s' s'' : t) :=
-   Raw.lt_trans (s:=s) (s':=s') (s'':=s'').
- Definition lt_not_eq (s s' : t) := Raw.lt_not_eq (sorted s) (sorted s').
+ Definition lt (s s'  t) := Raw.lt s s'.
+ Definition lt_trans (s s' s''  t) :=
+   Raw.lt_trans (s=s) (s':=s') (s'':=s'').
+ Definition lt_not_eq (s s'  t) := Raw.lt_not_eq (sorted s) (sorted s').
 
- Definition compare : forall s s' : t, Compare lt eq s s'.
+ Definition compare  forall s s' : t, Compare lt eq s s'.
  Proof.
  intros; elim (Raw.compare (sorted s) (sorted s'));
   [ constructor 1 | constructor 2 | constructor 3 ]; 
